examples/Toddler.v
@@ -39,7 +39,7 @@ Inductive factR : W -> W -> Prop :=
 | FR0 : factR 0 1
 | FRS : forall w r : W, w <> 0 -> factR (w ^- $1) r -> factR w (w ^* r).
 
-Lemma FR0' : forall w : W, w = 0 -> factR w 1.
+Lemma FR0' : forall w : W, w = 0 -> factR w $1.
   intros; subst; apply FR0.
 Qed.
 
@@ -73,7 +73,7 @@ Eval compute in compile fact.
 Lemma times_1 : forall (n m x : W), factR n x
   -> m = $1 ^* x
   -> factR n m.
-  intros; subst; replace ($1 ^* x) with x by W_eq; auto.
+  intros; subst. replace ($1 ^* x) with x by W_eq. auto.
 Qed.
 
 Hint Resolve times_1.
